coq/common/lemmas/exh.v
@@ -1,0 +1,69 @@
+(* =================================================== *)
+(* Properties of exhaustedness *)
+(* =================================================== *)
+
+Require Import common.obj.
+Require Import common.obj2.
+Require Import common.ctx.
+Require Import common.tp.
+Require Import Coq.Arith.PeanoNat.
+Require Import common.mult.lin_aff.
+Require Import Coq.Program.Equality.
+
+(* --------------------------------------------------- *)
+(* Pruning lemmas *)
+(* --------------------------------------------------- *)
+
+(* "Prune" LF context to remove dependencies *)
+
+(* Prune exh lemma *)
+Lemma prune_exh :
+  forall {N : nat} (delta : lctx N) (x : obj) (A : tp) (alpha : mult),
+    exh (cons N delta x A alpha) ->
+    exh delta.
+Proof.
+  intros N delta x A alpha H.
+  dependent destruction H.
+  exact H.
+Qed.
+
+
+Lemma exh_lookup :
+  forall {N : nat} (delta delta' : lctx N) (n : nat)
+         (X Y : obj) (A B : tp) (alpha beta : mult),
+    exh delta ->
+    upd delta n X Y A B alpha beta delta' ->
+    unr alpha.
+Proof.
+  intros N delta delta' n X Y A B alpha beta H_exh H_upd.
+  induction H_upd.
+  - (* Case upd_t *)
+    dependent destruction H_exh.
+    assumption.
+  - (* Case upd_n *)
+    dependent destruction H_exh.
+    apply IHH_upd; assumption.
+Qed.
+
+(* Changing type of an element of an exhausted context preserves exhaustedness *)
+(* (1) If exh(Δ) and unr(β), then exh(Δ[x :α A ↦ₙ y :β B])  *)
+(* (2) If exh(Δ), then exh(Δ[x :α A ↦ₙ y :α B]) [corollary of (1) and exh_lookup] *)
+
+
+Lemma exh_changetp :
+  forall {N : nat} (delta delta' : lctx N) (n : nat)
+         (X Y : obj) (A B : tp) (alpha beta : mult),
+    exh delta ->
+    unr beta ->
+    upd delta n X Y A B alpha beta delta' ->
+    exh delta'.
+Admitted.
+
+
+Lemma exh_changetp_cor :
+  forall {N : nat} (delta delta' : lctx N) (n : nat)
+         (X Y : obj) (A B : tp) (alpha : mult),
+    exh delta ->
+    upd delta n X Y A B alpha alpha delta' ->
+    exh delta'.
+Admitted.
