coq/common/lemmas/obj2_lemma.v
@@ -1,0 +1,22 @@
+(* =================================================== *)
+(* Further properties of objects *)
+(* (assuming the type obj is uninhabited) *)
+(* =================================================== *)
+
+Require Import common.obj.
+Require Import common.obj2.
+Require Import common.ctx.
+
+(* For any objects M and N, either M = N or M ≠ N *)
+
+Lemma comp_obj :
+  forall (M N : obj) (psi : ctx),
+    InCtx psi M ->
+    InCtx psi N ->
+    CompareObjs psi M N.
+Admitted.
+
+Lemma prune_obj :
+  forall (psi : ctx) (x p : obj),
+    obj_eq p x -> False -> PruneObj (extend x psi) (fun _ => p).
+Admitted.
