coq/common/lemmas/varctx.v
@@ -1,0 +1,49 @@
+(* =================================================== *)
+(* Properties of VarCtx predicate *)
+(* =================================================== *)
+
+Require Import common.ctx.
+Require Import common.obj.
+Require Import common.obj2.
+Require Import common.tp.
+Require Import Coq.Arith.PeanoNat.
+Require Import common.mult.lin_aff.
+
+(* If VarCtx [Ψ ⊢ Δ] and x ∈ Δ, then x is a parameter variable from Ψ *)
+Lemma varctx_isvar :
+  forall {N : nat} (psi : ctx) (delta delta' : lctx N) (n : nat)
+         (X X' : obj) (A A' : tp) (alpha alpha' : mult),
+    VarCtx psi delta ->
+    upd delta n X X' A A' alpha alpha' delta' ->
+    IsVar psi X.
+Admitted.
+
+(* Extend VarCtx judgment with new variable of type obj *)
+Lemma varctx_ext :
+  forall {N : nat} (psi : ctx) (delta : lctx N) (x : obj),
+    VarCtx psi delta ->
+    VarCtx (extend x psi) delta.
+Admitted.
+
+(* Extending a context with a fresh variable preserves VarCtx predicate *)
+Lemma varctx_extcons :
+  forall {N : nat} (psi : ctx) (delta : lctx N) (x : obj) (A : tp) (alpha : mult),
+    VarCtx psi delta ->
+    VarCtx (extend x psi) (cons N delta x A alpha).
+Admitted.
+
+(* If VarCtx [Ψ ⊢ Δ] and Δ₁ ⋈ Δ₂ = Δ, then VarCtx [Ψ ⊢ Δ₁] *)
+Lemma varctx_merge :
+  forall {N : nat} (psi : ctx) (delta delta1 delta2 : lctx N),
+    VarCtx psi delta ->
+    merge delta1 delta2 delta ->
+    VarCtx psi delta1.
+Admitted.
+
+(* If VarCtx [Ψ ⊢ Δ] and Δ₁ ⋈ Δ₂ = Δ, then VarCtx [Ψ ⊢ Δ₂] *)
+Lemma varctx_merge_r :
+  forall {N : nat} (psi : ctx) (delta delta1 delta2 : lctx N),
+    VarCtx psi delta ->
+    merge delta1 delta2 delta ->
+    VarCtx psi delta2.
+Admitted.
