coq/common/lemmas/wf.v
@@ -1,0 +1,41 @@
+(* =================================================== *)
+(* Properties of Wf predicate *)
+(* =================================================== *)
+
+Require Import common.ctx.
+Require Import common.obj.
+Require Import common.tp.
+Require Import Coq.Arith.PeanoNat.
+Require Import common.mult.lin_aff.
+
+(* Proving properties about well-formedness requires a series of auxilliary technical lemmas about *)
+(* context membership like the following. *)
+
+(* Adjusting Arguments *)
+Arguments lookup_n X {N} delta.
+Arguments lookn {N} A alpha delta delta' X n _.
+Arguments upd_t {N} delta X X' A A' alpha alpha'.
+Arguments upd_n {N} delta delta' n X X' Y A A' B alpha alpha' beta _.
+
+(* Auxiliary lemma: refl_top *)
+Lemma refl_top {N : nat} (delta : lctx N) (X : obj) (A : tp) (alpha : mult) :
+  upd (cons N delta X A alpha) (S N) X X A A alpha alpha (cons N delta X A alpha).
+Proof.
+  apply upd_t.
+Qed.
+
+(* Main lemma: look_top *)
+Lemma look_top {N : nat} (delta : lctx N) (X : obj) (A : tp) (alpha : mult) :
+  lookup_n X (cons N delta X A alpha).
+Proof.
+  apply lookn with (A := A) (alpha := alpha) (delta' := cons N delta X A alpha) (n := S N).
+  - apply refl_top.
+Qed.
+
+(* --------------------------------------------------- *)
+(* Main properties of context well-formedness *)
+(* --------------------------------------------------- *)
+
+(* If Wf [Ψ ⊢ Δ] and x ∈ Δ, then x is a parameter variable from Ψ *)
+
+
